@prefix rdf: <http://www.w3.org/1999/02/22-rdf-syntax-ns#> .
@prefix rdfs: <http://www.w3.org/2000/01/rdf-schema#> . 
@prefix owl: <http://www.w3.org/2002/07/owl#> .
@prefix dct: <http://purl.org/dc/terms/> .
@prefix skos: <http://www.w3.org/2004/02/skos/core#> .
@prefix openwemi: <https://dcmi.github.io/openwemi/ns#> .

openwemi: a owl:Ontology ;
   dct:title "OpenWEMI vocabulary" ;
   dct:creator "Dublin Core Metadata Initiative, OpenWEMI Working Group" ;
   dct:date "2024/01/19" ;
   dct:description "OpenWEMI is a minimally constrained vocabulary for describing created resources using the concepts of Work, Expression, Manifestation, Item." .


openwemi:Endeavor
  a rdfs:Class, owl:Class ;
  rdfs:label "Endeavor"@en ;
  skos:definition "A creation."@en ;
  rdfs:isDefinedBy openwemi: .
  
openwemi:Work
  a rdfs:Class, owl:Class ;
  rdfs:label "Work"@en ;
  skos:definition "An abstract notion of an artistic or intellectual creation."@en ;
  rdfs:isDefinedBy openwemi: ;
  dct:description "A work is an abstraction that represents the concepts behind a creation. Each metadata community will have a different definition of Work, but it should be the broadest definition of the creations being described."@en ;
  rdfs:subClassOf openwemi:Endeavor .

openwemi:Expression
  a rdfs:Class, owl:Class ;
  rdfs:label "Expression"@en ;
  skos:definition "A perceivable form of the creation."@en ;
  rdfs:isDefinedBy openwemi: ;
  dct:description "Creations are made tangible through some kind of expression, such as text, sound, or a visual form. There may be more than one expression of a work of the same type or of different types."@en ;
  rdfs:subClassOf openwemi:Endeavor .

openwemi:Manifestation
  a rdfs:Class, owl:Class ;
  rdfs:label "Manifestation"@en ;
  skos:definition "The physical embodiment of a creation."@en ;
  rdfs:isDefinedBy openwemi: ;
  dct:description "A manifestation is a creation that has been realized in some physical or digital form. A manifestation may be a single realization or a realization that is produced in multiple copies such as the publication of a music compact disk or the manufacture of a shirt."@en ;
  rdfs:subClassOf openwemi:Endeavor .
  
openwemi:Item
  a rdfs:Class, owl:Class ;
  rdfs:label "Item"@en ;
  skos:definition "An exemplar of a creation."@en ;
  rdfs:isDefinedBy openwemi: ;
  dct:description "An Item is a single instance of the creation, something that can have a place on a shelf or a location online."@en ;
  rdfs:subClassOf openwemi:Endeavor .
      
openwemi:relatedWork
  a rdf:Property ;
  rdfs:label "related Work"@en ;
  skos:definition "A Work that is related in some way to another Work."@en ;
  rdfs:isDefinedBy openwemi: ;
  rdfs:subPropertyOf dct:relation ;
  rdfs:domain openwemi:Work ;
  dct:description "This provides a non-specific relationship between two Works. The specific relationship type can be defined as a sub-property of relatedWork."@en ;
  rdfs:range openwemi:Work .

openwemi:relatedExpression
  a rdf:Property ;
  rdfs:label "related Expression"@en ;
  skos:definition "An Expression that is related in some way to another Expression."@en ;
  rdfs:isDefinedBy openwemi: ;
  rdfs:subPropertyOf dct:relation ;
  rdfs:domain openwemi:Expression ;
  dct:description "This provides a non-specific relationship between two Expressions. The specific relationship type can be defined as a sub-property of relatedExpression."@en ;
  rdfs:range openwemi:Expression .

openwemi:relatedManifestation
  a rdf:Property ;
  rdfs:label "related Manifestation"@en ;
  skos:definition "A Manifestation that is related in some way to another Manifestation."@en ;
  rdfs:isDefinedBy openwemi: ;
  rdfs:subPropertyOf dct:relation ;
  rdfs:domain openwemi:Manifestation ;
  dct:description "This provides a non-specific relationship between two Manifestations. The specific relationship type can be defined as a sub-property of relatedManifestation."@en ;
  rdfs:range openwemi:Manifestation .

openwemi:relatedItem
  a rdf:Property ;
  rdfs:label "related Item"@en ;
  skos:definition "An Item that is related in some way to another Item."@en ;
  rdfs:isDefinedBy openwemi: ;
  rdfs:subPropertyOf dct:relation ;
  rdfs:domain openwemi:Item ;
  dct:description "This provides a non-specific relationship between two Items. The specific relationship type can be defined as a sub-property of relatedItem."@en ;
  rdfs:range openwemi:Item .

openwemi:expresses
  a rdf:Property ;
  rdfs:label "expresses"@en ;
  skos:definition "An Endeavor that expresses a Work."@en ;
  rdfs:isDefinedBy openwemi: ;
  rdfs:subPropertyOf dct:relation ;
  rdfs:domain openwemi:Expression ;
  dct:description "A relationship asserted from an Expression to a Work that it expresses."@en ;
  rdfs:range openwemi:Work .

 openwemi:expressedBy
  a rdf:Property ;
  rdfs:label "expressed by"@en ;
  skos:definition "An Expression of a Work."@en ;
  owl:inverseOf openwemi:expresses ;
  rdfs:isDefinedBy openwemi: ;
  rdfs:subPropertyOf dct:relation ;
  rdfs:domain openwemi:Work ;
  dct:description "A relationship asserted from a Work to an Expression that expresses the Work."@en ;
  rdfs:range openwemi:Expression . 

openwemi:manifests
  a rdf:Property ;
  rdfs:label "manifests"@en ;
  skos:definition "An Endeavor that manifests an Expression or a Work."@en ;
  rdfs:isDefinedBy openwemi: ;
  rdfs:subPropertyOf dct:relation ;
  rdfs:domain openwemi:Manifestation ;
  dct:description "A relationship asserted from a Manifestation to an Expression or a Work."@en ;
  rdfs:range [
    a owl:Class ;
    owl:unionOf (
      openwemi:Work 
      openwemi:Expression
    )
  ] .

openwemi:manifestedBy
  a rdf:Property ;
  rdfs:label "manifested by"@en ;
  skos:definition "A Manifestation of a Work or an Expression."@en ;
  owl:inverseOf openwemi:manifests ;
  rdfs:isDefinedBy openwemi: ;
  rdfs:subPropertyOf dct:relation ;
  dct:description "A relationship asserted from a Work or an Expression to a Manifestation."@en ;
  rdfs:domain [
      a owl:Class ;
      owl:unionOf (
       openwemi:Work 
       openwemi:Expression
     )
    ] ;
  rdfs:range openwemi:Manifestation . 

openwemi:instantiates
  a rdf:Property ;
  rdfs:label "instantiates"@en ;
  skos:definition "An Endeavor that instantiates a Manifestation, an Expression or a Work."@en ;
  rdfs:isDefinedBy openwemi: ;
  rdfs:subPropertyOf dct:relation ;
  rdfs:domain openwemi:Item ;
  dct:description "A relationship asserted from an Item to a Manifestation, an Expression, or a Work."@en ;
  rdfs:range [
    a owl:Class ;
    owl:unionOf (
      openwemi:Work
      openwemi:Expression
      openwemi:Manifestation
    )
  ] .

openwemi:instantiatedBy
  a rdf:Property ;
  rdfs:label "instantiated by"@en ;
  skos:definition "An instantiation of a Manifestation, an Expression or a Work."@en ;
  owl:inverseOf openwemi:instantiates ;
  rdfs:isDefinedBy openwemi: ;
  rdfs:subPropertyOf dct:relation ;
  dct:description "A relationship asserted from a Work, an Expression, or a Manifestation to an Item."@en ;
  rdfs:domain [
      a owl:Class ;
      owl:unionOf (
       openwemi:Work 
       openwemi:Expression
       openwemi:Manifestation
     )
    ] ;
  rdfs:range openwemi:Item .

openwemi:commonEndeavor
    a rdf:Property ;
    rdfs:isDefinedBy openwemi: ;
    rdfs:label "common Endeavor"@en ;
    skos:definition "Relates any two resources that are or contain the same endeavor." ;
    dct:description "commonEndeavour is intended to define a relationship between two resources that may or may not be modeled as . This makes it possible to assert that a resource modeled using a vocabulary that does not use the  entity model explicitly is describing the same Work, Expression, Manifestation, and/or Item as another resource."@en ;
    owl:equivalentProperty <http://open.vocab.org/terms/commonEndeavour> .
    
openwemi:commonWork
    a rdf:Property ;
    rdfs:isDefinedBy openwemi: ;
    rdfs:label "common Work"@en ;
    skos:definition "Relates any two resources that are or contain the same Work." ;
    dct:description "commonWork is intended to define a relationship between two resources that may or may not be modeled as OpenWEMI. This makes it possible to assert that a resource modeled using a vocabulary that does not use the OpenWEMI entity model explicitly is describing the same Work as another resource."@en ;
        owl:equivalentProperty <http://open.vocab.org/terms/commonWork> .
        
openwemi:commonExpression
    a rdf:Property ;
    rdfs:isDefinedBy openwemi: ;
    rdfs:label "common Expression"@en ;
    skos:definition "Relates any two resources that are or contain the same Expression." ;
    dct:description "commonExpression is intended to define a relationship between two resources that may or may not be modeled as OpenWEMI. This makes it possible to assert that a resource modeled using a vocabulary that does not use the OpenWEMI entity model explicitly is describing the Expression as another resource."@en ;
    owl:equivalentProperty <http://open.vocab.org/terms/commonExpression> .

openwemi:commonManifestation
    a rdf:Property ;
    rdfs:isDefinedBy openwemi: ;
    rdfs:label "common Manifestation"@en ;
    skos:definition "Relates any two resources that are or contain the same Manifestation." ;
    dct:description "commonManifestation is intended to define a relationship between two resources that may or may not be modeled as OpenWEMI. This makes it possible to assert that a resource modeled using a vocabulary that does not use the OpenWEMI entity model explicitly is describing the same Manifestation as another resource."@en ;
    owl:equivalentProperty <http://open.vocab.org/terms/commonManifestation> .

openwemi:commonItem
    a rdf:Property ;
    rdfs:isDefinedBy openwemi: ;
    rdfs:label "common Item"@en ;
    skos:definition "Relates any two resources that are or contain the same Item." ;
    dct:description "commonItem is intended to define a relationship between two resources that may or may not be modeled as OpenWEMI. This makes it possible to assert that a resource modeled using a vocabulary that does not use the OpenWEMI entity model explicitly is describing the same Item as another resource."@en ;
    owl:equivalentProperty <http://open.vocab.org/terms/commonItem> .
