@prefix rdf: <http://www.w3.org/1999/02/22-rdf-syntax-ns#> .
@prefix rdfs: <http://www.w3.org/2000/01/rdf-schema#> . 
@prefix owl: <http://www.w3.org/2002/07/owl#> .
@prefix dct: <http://purl.org/dc/terms/> .
@prefix skos: <http://www.w3.org/2004/02/skos/core#> .
@prefix openwemi: <https://ns.dublincore.org/openwemi/> .
@prefix quilt: <https://example.com/quilt/> .

quilt: a owl:Ontology ;
   dct:title "Quilt vocabulary" ;
   dct:description "This quilt vocabulary is subclassed to OpenWEMI to make use of the concepts of Work, Expression, Manifestation, Item." .
  
quilt:DesignConcept
  a rdfs:Class, owl:Class ;
  rdfs:label "Design concept"@en ;
  rdfs:comment "A conceptual design for a quilt."@en ;
  rdfs:isDefinedBy quilt: ;
  dct:description "A conceptual design, possibly, but not necessarily, based on a block pattern."@en ;
  rdfs:subClassOf openwemi:Work .

quilt:DesignDiagram
  a rdfs:Class, owl:Class ;
  rdfs:label "Design diagram"@en ;
  rdfs:comment "A diagram that shows the quilt design."@en ;
  rdfs:isDefinedBy quilt: ;
  dct:description "The quilt design diagram is usually in the form of a drawing that gives the structure of the quilt and/or quilt blocks. Different expressions can indicate options such as quilt size, addition of borders, and fabric suggestions."@en ;
  rdfs:subClassOf openwemi:Expression .

quilt:Pattern
  a rdfs:Class, owl:Class ;
  rdfs:label "Quilt pattern"@en ;
  rdfs:comment "A quilt pattern that is available in some tangible form, such as printed in a document or for download."@en ;
  rdfs:isDefinedBy quilt: ;
  dct:description "The quilt:Pattern generally includes all of the information needed for a person to make the quilt. There are fabric needs (yardage), cutting instructions, and piecing instructions. There may also be size options, fabric suggestions, and other useful information."@en ;
  rdfs:subClassOf openwemi:Manifestation .
  
quilt:CompletedQuilt
  a rdfs:Class, owl:Class ;
  rdfs:label "Completed quilt"@en ;
  rdfs:comment "An actual (physical) quilt that 1) instantiates the quilt:Expression and 2) may be the direct application of a quilt:Manifestation."@en ;
  rdfs:isDefinedBy quilt: ;
  dct:description "The quilt:CompletedQuilt may be a direct creation following the quilt:Pattern, but variations visible in the quilt:CompletedQuilt do not generally create a new work. Such variations may be in terms of color and fabric choice, and use of borders. Other variations, such as using a different quilt block design, may be considered a new work."@en ;
  rdfs:subClassOf openwemi:Item .
     

quilt:designOf
  a rdf:Property ;
  rdfs:label "Design of"@en ;
  rdfs:comment "An Endeavor that expresses a quilt:DesignConcept."@en ;
  rdfs:isDefinedBy quilt: ;
  rdfs:subPropertyOf openwemi:expresses ;
  rdfs:domain quilt:Expression ;
  dct:description "A relationship asserted from a DesignDiagram to the DesignConcept that it describes."@en ;
  rdfs:range quilt:DesignConcept .

quilt:patternOf
  a rdf:Property ;
  rdfs:label "Pattern of"@en ;
  rdfs:comment "A quilt:Pattern that implements a quilt:DesignPattern."@en ;
  rdfs:isDefinedBy quilt: ;
  rdfs:subPropertyOf openwemi:manifests ;
  rdfs:domain quilt:DesignPattern ;
  dct:description "A relationship asserted from a quilt:Pattern to a quilt:DesignDiagram."@en ;
  rdfs:range quilt:Pattern . 

quilt:creates
  a rdf:Property ;
  rdfs:label "Creates"@en ;
  rdfs:comment "A completed quilt based on a quilt pattern."@en ;
  rdfs:isDefinedBy quilt: ;
  rdfs:subPropertyOf openwemi:instantiates ;
  rdfs:domain quilt:Item ;
  dct:description "A completed quilt for this quilt pattern."@en ;
  rdfs:range quilt:CompletedQuilt.

  quilt:relatedDesignConcept
    a rdf:Property ;
    rdfs:label "Related design"@en ;
    rdfs:comment "A quilt:DesignConcept that is related in some way to another quilt:DesignConcept."@en ;
    rdfs:isDefinedBy quilt: ;
    rdfs:subPropertyOf openwemi:relatedWork ;
    rdfs:domain quilt:DesignConcept ;
    dct:description "This provides a non-specific relationship between two quilt:DesignConcepts. If needed, the specific relationship type can be defined as a sub-property of quilt:relatedDesignConcept."@en ;
    rdfs:range quilt:DesignConcept .

  quilt:relatedDesignDiagram
    a rdf:Property ;
    rdfs:label "related Expression"@en ;
    rdfs:comment "A quilt:DesignDiagram that is related in some way to another quilt:DesignDiagram."@en ;
    rdfs:isDefinedBy quilt: ;
    rdfs:subPropertyOf openwemi:relatedExpression ;
    rdfs:domain quilt:Expression ;
    dct:description "This provides a non-specific relationship between two DesignDiagrams. If needed, the specific relationship type can be defined as a sub-property of relatedDesignDiagram."@en ;
    rdfs:range quilt:DesignDiagram .

  quilt:relatedPattern
    a rdf:Property ;
    rdfs:label "related Pattern"@en ;
    rdfs:comment "A quilt:Pattern that is related in some way to another quilt:Pattern."@en ;
    rdfs:isDefinedBy quilt: ;
    rdfs:subPropertyOf openwemi:relatedManifestation ;
    rdfs:domain quilt:Manifestation ;
    dct:description "This provides a non-specific relationship between two Patterns. If needed, the specific relationship type can be defined as a sub-property of relatedPattern."@en ;
    rdfs:range quilt:Pattern .

  quilt:relatedCompletedQuilt
    a rdf:Property ;
    rdfs:label "related Item"@en ;
    rdfs:comment "A quilt:CompletedQuilt that is related in some way to another quilt:CompletedQuilt."@en ;
    rdfs:isDefinedBy quilt: ;
    rdfs:subPropertyOf openwemi:relatedItem ;
    rdfs:domain quilt:Item ;
    dct:description "This provides a non-specific relationship between two quilt:CompletedQuilt. The specific relationship type can be defined as a sub-property of quilt:CompletedQuilt."@en ;
    rdfs:range quilt:CompletedQuilt .